rupicola/io/IO.fst
@@ -4,10 +4,11 @@ module IO
 open Trace
 open STLC
 
+open FStar.Tactics
+
 noeq
 type io (a:Type u#a) : Type u#a =
 | Call : o:io_ops -> args:io_args o -> (io_res o args -> io a) -> io a
-//| PartialCall : (pre:pure_pre) -> cont:((squash pre) -> io u#a a) -> io a
 | Return : a -> io a
 
 let io_return (#a:Type) (x:a) : io a =
@@ -25,11 +26,17 @@ let rec io_bind
       Call o args (fun i ->
         io_bind #a #b (fnc i) k)
 
-let read () : io (resexn bool) =
-  Call ORead () Return
+let openfile (fnm:bool) : io (resexn file_descr) =
+  Call OOpen fnm Return
 
-let write (x:bool) : io (resexn unit) =
+let read (fd:file_descr) : io (resexn bool) =
+  Call ORead fd Return
+
+let write (x:file_descr * bool) : io (resexn unit) =
   Call OWrite x Return
+
+let close (fd:file_descr) : io (resexn unit) =
+  Call OClose fd Return
 
 let op_wp (o:io_ops) (args:io_args o) : hist (io_res o args) =
   to_hist
@@ -44,25 +51,24 @@ let rec theta #a (m:io a) : hist a =
 let theta_monad_morphism_ret x =
   assert (theta (return x) == hist_return x) by (FStar.Tactics.compute ())
 
-let theta_monad_morphism_bind m k = admit ()
+let theta_monad_morphism_bind m k =
+  admit () (** Cezar: should be double. existing proof in sciostar/DMFree.fst **)
+
+let io_bind_equivalence (#a #b:Type) (k k':a -> io b) (m:io a) :
+  Lemma (requires forall x. k x == k' x)
+        (ensures theta (io_bind m k) `hist_equiv` theta (io_bind m k')) =
+  admit () (** Cezar: Is induction on m enough? **)
 
 let wp2p_theta_bind m k =
   theta_monad_morphism_bind m k
 
-let io_bind_equivalence (#a #b:Type) (k k':a -> io b) (m:io a) :
-  Lemma (requires forall x. k x == k' x)
-        (ensures theta (io_bind m k) `hist_equiv` theta (io_bind m k')) = admit ()
+let lem_theta_read arg res h =
+  assert (thetaP (read arg) h [EvRead arg res] res) by (compute ())
 
-let lem_theta_read (x:io_res ORead ()) (h:history) (lt:local_trace h) :
-  Lemma (requires lt == [EvRead () x])
-        (ensures wp2p (theta (read ())) h lt x) =
-  assert (theta (read ()) == (fun (h:history) (p:hist_post h (resexn bool)) -> (forall (lt:local_trace h) (r:resexn bool). lt == [EvRead () r] ==> p (lt @ []) r))) by (assert (lt @ []) == lt; FStar.Tactics.compute ())
+let lem_theta_write arg res h =
+  assert (thetaP (write arg) h [EvWrite arg res] res) by (compute ())
 
-let lem_theta_write (b:bool) (x:io_res OWrite b) (h:history) (lt:local_trace h) :
-  Lemma (requires lt == [EvWrite b x])
-        (ensures wp2p (theta (write b)) h lt x) =
-  assert (theta (write b) == (fun (h:history) (p:hist_post h (resexn unit)) -> (forall (lt:local_trace h) (r:resexn unit). lt == [EvWrite b r] ==> p (lt @ []) r))) by (assert (lt @ []) == lt; FStar.Tactics.compute ())
-
+(**
 let rec get_lt (h h':history) (lt:local_trace h) : Tot (local_trace h') (decreases lt) =
   match lt with
   | [] -> []
@@ -70,28 +76,32 @@ let rec get_lt (h h':history) (lt:local_trace h) : Tot (local_trace h') (decreas
     match ev with
     | EvRead args res -> begin
       // here we will need to check compatability of ev with h' and either return Inl or Inr of unit
-      assume (test_event h' ev); 
+      assume (test_event h' ev);
       assume (well_formed_local_trace (ev::h) tl);
-      assume (forall (lt':local_trace (ev::h')). well_formed_local_trace h' (ev::lt')); 
+      assume (forall (lt':local_trace (ev::h')). well_formed_local_trace h' (ev::lt'));
       ev :: (get_lt (ev::h) (ev::h') tl)
       end
     | EvWrite args res -> begin
       // here we will need to check compatability of ev with h' and either return Inl or Inr of unit
-      assume (test_event h' ev); 
+      assume (test_event h' ev);
       assume (well_formed_local_trace (ev::h) tl);
       assume (forall (lt':local_trace (ev::h')). well_formed_local_trace h' (ev::lt'));
       ev :: (get_lt (h++[ev]) (h'++[ev]) tl)
       end
     end
+**)
 
 // (lt == [] ==> (get_lt h h' []) == [])
 
+(*
 let get_lt_correct (h h':history) (lt:local_trace h) :
   Lemma ((lt == [] ==> (get_lt h h' []) == []) /\
          (forall (lt1:local_trace h) (lt2:local_trace (h++lt1)). lt == (lt1 @ lt2) ==> (get_lt h h' (lt1 @ lt2)) == (get_lt h h' lt1) @ (get_lt (h++lt1) (h'++lt1) lt2))) = admit ()
+*)
 
 // x ( lt1 @ lt2) == x lt1 @ x lt2
 
+(*
 let rec theta_monotonic_hist (m:io 'a) :
 Lemma (forall h h' (p':hist_post h' 'a). (theta m h' p' ==> theta m h (fun lt res -> p' (get_lt h h' lt) res))) =
   match m with
@@ -127,7 +137,9 @@ Lemma (forall h h' (p':hist_post h' 'a). (theta m h' p' ==> theta m h (fun lt re
       end
     end
     end
+*)
 
+(*
 let theta_history_independence #a (m:io a) (h h':history) (lt:local_trace h) (fs_r:a) :
   Lemma (requires wp2p (theta m) h lt fs_r)
         (ensures wp2p (theta m) h' (get_lt h h' lt) fs_r) =
@@ -140,8 +152,9 @@ let theta_history_independence #a (m:io a) (h h':history) (lt:local_trace h) (fs
       assert (p' (get_lt h h' lt) fs_r)
     end
   end
+*)
 
-(* DEFINITION UNFOLDING 
+(* DEFINITION UNFOLDING
 assert (theta m h' p' == theta (Call o args k) h' p');
         assert (theta m h (fun lt res -> p' (get_lt h h' lt) res) == theta (Call o args k) h (fun lt res -> p' (get_lt h h' lt) res));
         assert (theta (Call o args k) h' p' == hist_bind (op_wp o args) (fun r -> theta (k r)) h' p') by (FStar.Tactics.compute ());
@@ -208,7 +221,7 @@ Lemma (forall h h' (p':hist_post h' 'a). (theta m h' p' ==> theta m h (fun lt re
     assert (forall p. (theta m) h p ==> p [] x);
     introduce forall (p':hist_post h' a). (theta m) h' p' ==> p' lt' fs_r with begin
       introduce (theta m) h' p' ==> p' lt' fs_r with _. begin
-      
+
         let p : hist_post h a = fun lt res -> p' (get_lt h h' lt) res in
         eliminate forall p. (theta m) h p ==> p lt fs_r with p;
         assert ((theta m) h' p');
@@ -217,7 +230,7 @@ Lemma (forall h h' (p':hist_post h' 'a). (theta m h' p' ==> theta m h (fun lt re
         assert (p lt fs_r);
         assert (p' (get_lt h h' lt) fs_r);
         //assert ((get_lt h h' lt) == lt');
-  
+
         admit ()
         //assert ((theta m) h p ==> p lt fs_r);
         //admit ()
@@ -232,7 +245,7 @@ Lemma (forall h h' (p':hist_post h' 'a). (theta m h' p' ==> theta m h (fun lt re
   | Call o args k -> admit ()
   (*introduce forall (p':hist_post h' a). (theta m) h' p' ==> p' lt' fs_r with begin
     introduce (theta m) h' p' ==> p' lt' fs_r with _. begin
-      
+
       let p : hist_post h a = fun lt res -> p' (get_lt h h' lt) res in
       eliminate forall p. (theta m) h p ==> p lt fs_r with p;
       assert ((theta m) h' p');
@@ -256,7 +269,7 @@ Lemma (forall h h' (p':hist_post h' 'a). (theta m h' p' ==> theta m h (fun lt re
     assert (forall p. (theta m) h p ==> p [] x);
     introduce forall (p':hist_post h' a). (theta m) h' p' ==> p' lt' fs_r with begin
       introduce (theta m) h' p' ==> p' lt' fs_r with _. begin
-      
+
         let p : hist_post h a = fun lt res -> p' (get_lt h h' lt) res in
         eliminate forall p. (theta m) h p ==> p lt fs_r with p;
         assert ((theta m) h' p');
@@ -273,7 +286,7 @@ Lemma (forall h h' (p':hist_post h' 'a). (theta m h' p' ==> theta m h (fun lt re
   | Call o args k -> admit ()
   (*introduce forall (p':hist_post h' a). (theta m) h' p' ==> p' lt' fs_r with begin
     introduce (theta m) h' p' ==> p' lt' fs_r with _. begin
-      
+
       let p : hist_post h a = fun lt res -> p' (get_lt h h' lt) res in
       eliminate forall p. (theta m) h p ==> p lt fs_r with p;
       assert ((theta m) h' p');
