rupicola/io/IO.fsti
@@ -23,8 +23,10 @@ val io_bind
   (k : a -> io b) :
   io b
 
-val read () : io (resexn bool)
-val write (x:bool) : io (resexn unit)
+val openfile : bool -> io (resexn file_descr)
+val read : file_descr -> io (resexn bool)
+val write : file_descr * bool -> io (resexn unit)
+val close : file_descr -> io (resexn unit)
 
 let return = io_return
 let (let!@) = io_bind
@@ -37,51 +39,70 @@ val theta_monad_morphism_ret (x:'a) :
 val theta_monad_morphism_bind (m:io 'a) (k:'a -> io 'b) :
   Lemma (theta (io_bind m k) `hist_equiv` hist_bind (theta m) (fun x -> theta (k x)))
 
-val wp2p_theta_bind (m:io 'a) (k:'a -> io 'b) :
-  Lemma (forall h.
-         wp2p (hist_bind (theta m) (fun x -> theta (k x))) h
-         `hist_post_equiv`
-         wp2p (theta (io_bind m k)) h)
-
 val io_bind_equivalence #a #b (k k':a -> io b) (m:io a) :
   Lemma (requires forall x. k x == k' x)
         (ensures theta (io_bind m k) `hist_equiv` theta (io_bind m k'))
 
-let lem_theta_return #a (x:a) (h:history) (lt:local_trace h) :
-  Lemma (requires lt == [])
-        (ensures wp2p (theta (return x)) h lt x) =
+let thetaP m = wp2p (theta m)
+
+val wp2p_theta_bind (m:io 'a) (k:'a -> io 'b) :
+  Lemma (forall h.
+         wp2p (hist_bind (theta m) (fun x -> theta (k x))) h (** Kind of ugly. Can we use hist_post_bind? **)
+         `hist_post_equiv`
+         thetaP (io_bind m k) h)
+
+(** Cezar: Trying to connect with hist_post_bind. Does not look like it holds.
+let lem_thetaP_bind #a #b (m:io a) (k:a -> io b) :
+  Lemma (forall h.
+         wp2p (hist_bind (theta m) (fun x -> theta (k x))) h
+        `hist_post_equiv`
+         hist_post_bind (thetaP m h) (fun lt r -> thetaP (k r) (h++lt))) =
+  assert (forall h.
+         wp2p (hist_bind (theta m) (fun x -> theta (k x))) h
+        `hist_post_equiv`
+         hist_post_bind (thetaP m h) (fun lt r -> thetaP (k r) (h++lt))) by (
+         norm [delta_only [`%hist_post_bind; `%thetaP; `%hist_bind; `%wp2p;
+         `%hist_post_bind'; `%hist_post_shift;`%hist_post_equiv;`%hist_post_ord]; iota];
+         let h = forall_intro () in
+         split ();
+         dump "H")
+**)
+
+val lem_theta_read (arg:io_args ORead) (res:io_res ORead arg) (h:history) :
+  Lemma (thetaP (read arg) h [EvRead arg res] res)
+
+val lem_theta_write (arg:io_args OWrite) (res:io_res OWrite arg) (h:history) :
+  Lemma (thetaP (write arg) h [EvWrite arg res] res)
+
+let thetaP_monad_morphism_return #a (x:a) (h:history) :
+  Lemma (thetaP (return x) h [] x) =
   theta_monad_morphism_ret x
 
-let lem_theta_bind #a #b (m:io a) (h:history) (lt2:local_trace h) (fs_r_m:a) (k:a -> io b) (lt3:local_trace (h++lt2)) (fs_r:b) (lt:local_trace h) :
-  Lemma (requires wp2p (theta m) h lt2 fs_r_m /\
-                  wp2p (theta (k fs_r_m)) (h++lt2) lt3 fs_r /\
-                  (lt == lt2 @ lt3))
-        (ensures wp2p (theta (io_bind m k)) h lt fs_r) =
+open FStar.Tactics
+
+let lem_thetaP_bind #a #b (m:io a) (h:history) (lt1:local_trace h) (fs_r_m:a) (k:a -> io b) (lt2:local_trace (h++lt1)) (fs_r:b) :
+  Lemma (requires thetaP m h lt1 fs_r_m /\
+                  thetaP (k fs_r_m) (h++lt1) lt2 fs_r)
+        (ensures thetaP (io_bind m k) h (lt1@lt2) fs_r) =
+  assume (wp2p (hist_bind (theta m) (fun x -> theta (k x))) h (lt1@lt2) fs_r);
   wp2p_theta_bind m k
 
-val lem_theta_read (x:io_res ORead ()) (h:history) (lt:local_trace h) :
-  Lemma (requires lt == [EvRead () x])
-        (ensures wp2p (theta (read ())) h lt x)
-
-val lem_theta_write (b:bool) (x:io_res OWrite b) (h:history) (lt:local_trace h) :
-  Lemma (requires lt == [EvWrite b x])
-        (ensures wp2p (theta (write b)) h lt x)
-
-val get_lt (h h':history) (lt:local_trace h) : Tot (local_trace h') 
+(**
+val get_lt (h h':history) (lt:local_trace h) : Tot (local_trace h')
 
 val theta_history_independence #a (m:io a) (h h':history) (lt:local_trace h) (fs_r:a) :
-  Lemma (requires wp2p (theta m) h lt fs_r)
-        (ensures wp2p (theta m) h' (get_lt h h' lt) fs_r) 
-  //(requires wp2p (theta m) h (get_lt h' h lt') fs_r)
-  //(ensures wp2p (theta m) h' lt' fs_r)
-  //      (ensures wp2p (theta m) h' (get_lt h h' lt) fs_r) 
+  Lemma (requires thetaP m h lt fs_r)
+        (ensures thetaP m h' (get_lt h h' lt) fs_r)**)
+  //(requires thetaP m) h (get_lt h' h lt') fs_r)
+  //(ensures thetaP m) h' lt' fs_r)
+  //      (ensures thetaP m) h' (get_lt h h' lt) fs_r)
 
 (*val theta_monotonic_hist #a #e #e' #h' #lt' (m:io a) (st:steps e e' h' lt') :
-  Lemma (forall h h' (p':hist_post h' a). theta m h' p' ==> theta m h (fun lt res -> p' (construct_local_trace st*) 
+  Lemma (forall h h' (p':hist_post h' a). theta m h' p' ==> theta m h (fun lt res -> p' (construct_local_trace st*)
 
 (*val theta_history_independence #a #e #e' (m:io a) (h h':history) (lt:local_trace h) (lt':local_trace h') (fs_r:a) (st':steps e e' h' lt') (st:steps e e' h lt) :
-  Lemma (requires wp2p (theta m) h (construct_local_trace st' h) fs_r)
-        (ensures wp2p (theta m) h' (construct_local_trace st h') fs_r)*)
+  Lemma (requires thetaP m) h (construct_local_trace st' h) fs_r)
+        (ensures thetaP m) h' (construct_local_trace st h') fs_r)*)
 
 (*let same_shape #h #h' (lt:local_trace h) (lt':local_trace h') : Type0 = lt == lt'
 
